sample_mark/dijkstra.v
@@ -15,146 +15,99 @@ Module Info.
   Definition normalized := true.
 End Info.
 
-Definition _Node : ident := 3%positive.
-Definition ___builtin_annot : ident := 12%positive.
-Definition ___builtin_annot_intval : ident := 13%positive.
-Definition ___builtin_bswap : ident := 6%positive.
-Definition ___builtin_bswap16 : ident := 8%positive.
-Definition ___builtin_bswap32 : ident := 7%positive.
-Definition ___builtin_bswap64 : ident := 38%positive.
-Definition ___builtin_clz : ident := 39%positive.
-Definition ___builtin_clzl : ident := 40%positive.
-Definition ___builtin_clzll : ident := 41%positive.
-Definition ___builtin_ctz : ident := 42%positive.
-Definition ___builtin_ctzl : ident := 43%positive.
-Definition ___builtin_ctzll : ident := 44%positive.
-Definition ___builtin_debug : ident := 56%positive.
-Definition ___builtin_fabs : ident := 9%positive.
-Definition ___builtin_fmadd : ident := 47%positive.
-Definition ___builtin_fmax : ident := 45%positive.
-Definition ___builtin_fmin : ident := 46%positive.
-Definition ___builtin_fmsub : ident := 48%positive.
-Definition ___builtin_fnmadd : ident := 49%positive.
-Definition ___builtin_fnmsub : ident := 50%positive.
-Definition ___builtin_fsqrt : ident := 10%positive.
-Definition ___builtin_membar : ident := 14%positive.
-Definition ___builtin_memcpy_aligned : ident := 11%positive.
-Definition ___builtin_nop : ident := 55%positive.
-Definition ___builtin_read16_reversed : ident := 51%positive.
-Definition ___builtin_read32_reversed : ident := 52%positive.
-Definition ___builtin_va_arg : ident := 16%positive.
-Definition ___builtin_va_copy : ident := 17%positive.
-Definition ___builtin_va_end : ident := 18%positive.
-Definition ___builtin_va_start : ident := 15%positive.
-Definition ___builtin_write16_reversed : ident := 53%positive.
-Definition ___builtin_write32_reversed : ident := 54%positive.
-Definition ___compcert_i64_dtos : ident := 23%positive.
-Definition ___compcert_i64_dtou : ident := 24%positive.
-Definition ___compcert_i64_sar : ident := 35%positive.
-Definition ___compcert_i64_sdiv : ident := 29%positive.
-Definition ___compcert_i64_shl : ident := 33%positive.
-Definition ___compcert_i64_shr : ident := 34%positive.
-Definition ___compcert_i64_smod : ident := 31%positive.
-Definition ___compcert_i64_smulh : ident := 36%positive.
-Definition ___compcert_i64_stod : ident := 25%positive.
-Definition ___compcert_i64_stof : ident := 27%positive.
-Definition ___compcert_i64_udiv : ident := 30%positive.
-Definition ___compcert_i64_umod : ident := 32%positive.
-Definition ___compcert_i64_umulh : ident := 37%positive.
-Definition ___compcert_i64_utod : ident := 26%positive.
-Definition ___compcert_i64_utof : ident := 28%positive.
-Definition ___compcert_va_composite : ident := 22%positive.
-Definition ___compcert_va_float64 : ident := 21%positive.
-Definition ___compcert_va_int32 : ident := 19%positive.
-Definition ___compcert_va_int64 : ident := 20%positive.
-Definition ___stringlit_1 : ident := 76%positive.
-Definition ___stringlit_2 : ident := 77%positive.
-Definition ___stringlit_3 : ident := 78%positive.
-Definition ___stringlit_4 : ident := 80%positive.
-Definition ___stringlit_5 : ident := 89%positive.
-Definition ___stringlit_6 : ident := 90%positive.
-Definition ___stringlit_7 : ident := 95%positive.
-Definition ___stringlit_8 : ident := 99%positive.
-Definition ___stringlit_9 : ident := 101%positive.
-Definition _adjustWeight : ident := 75%positive.
-Definition _argc : ident := 103%positive.
-Definition _argv : ident := 104%positive.
-Definition _before : ident := 98%positive.
-Definition _current : ident := 72%positive.
-Definition _del : ident := 66%positive.
-Definition _deleteNode : ident := 68%positive.
-Definition _dijkstra : ident := 96%positive.
-Definition _dist : ident := 92%positive.
-Definition _dst : ident := 84%positive.
-Definition _dst__1 : ident := 97%positive.
-Definition _free : ident := 58%positive.
-Definition _getPath : ident := 100%positive.
-Definition _getPaths : ident := 102%positive.
-Definition _graph : ident := 82%positive.
-Definition _head : ident := 67%positive.
-Definition _i : ident := 85%positive.
-Definition _j : ident := 86%positive.
-Definition _list : ident := 63%positive.
-Definition _main : ident := 105%positive.
-Definition _malloc : ident := 57%positive.
-Definition _minNode : ident := 71%positive.
-Definition _minVertex : ident := 70%positive.
-Definition _minWeight : ident := 69%positive.
-Definition _newHead : ident := 64%positive.
-Definition _newWeight : ident := 74%positive.
-Definition _next : ident := 4%positive.
-Definition _popMin : ident := 73%positive.
-Definition _pq : ident := 94%positive.
-Definition _prev : ident := 5%positive.
-Definition _print_graph : ident := 91%positive.
-Definition _print_list : ident := 81%positive.
-Definition _print_verts : ident := 79%positive.
-Definition _printf : ident := 61%positive.
-Definition _push : ident := 65%positive.
-Definition _rand : ident := 59%positive.
-Definition _random : ident := 87%positive.
-Definition _setup : ident := 88%positive.
-Definition _srand : ident := 60%positive.
-Definition _src : ident := 83%positive.
-Definition _time : ident := 62%positive.
-Definition _u : ident := 93%positive.
-Definition _vertex : ident := 1%positive.
-Definition _weight : ident := 2%positive.
-Definition _t'1 : ident := 106%positive.
-Definition _t'10 : ident := 115%positive.
-Definition _t'11 : ident := 116%positive.
-Definition _t'12 : ident := 117%positive.
-Definition _t'13 : ident := 118%positive.
-Definition _t'2 : ident := 107%positive.
-Definition _t'3 : ident := 108%positive.
-Definition _t'4 : ident := 109%positive.
-Definition _t'5 : ident := 110%positive.
-Definition _t'6 : ident := 111%positive.
-Definition _t'7 : ident := 112%positive.
-Definition _t'8 : ident := 113%positive.
-Definition _t'9 : ident := 114%positive.
+Definition ___builtin_annot : ident := 7%positive.
+Definition ___builtin_annot_intval : ident := 8%positive.
+Definition ___builtin_bswap : ident := 1%positive.
+Definition ___builtin_bswap16 : ident := 3%positive.
+Definition ___builtin_bswap32 : ident := 2%positive.
+Definition ___builtin_bswap64 : ident := 33%positive.
+Definition ___builtin_clz : ident := 34%positive.
+Definition ___builtin_clzl : ident := 35%positive.
+Definition ___builtin_clzll : ident := 36%positive.
+Definition ___builtin_ctz : ident := 37%positive.
+Definition ___builtin_ctzl : ident := 38%positive.
+Definition ___builtin_ctzll : ident := 39%positive.
+Definition ___builtin_debug : ident := 51%positive.
+Definition ___builtin_fabs : ident := 4%positive.
+Definition ___builtin_fmadd : ident := 42%positive.
+Definition ___builtin_fmax : ident := 40%positive.
+Definition ___builtin_fmin : ident := 41%positive.
+Definition ___builtin_fmsub : ident := 43%positive.
+Definition ___builtin_fnmadd : ident := 44%positive.
+Definition ___builtin_fnmsub : ident := 45%positive.
+Definition ___builtin_fsqrt : ident := 5%positive.
+Definition ___builtin_membar : ident := 9%positive.
+Definition ___builtin_memcpy_aligned : ident := 6%positive.
+Definition ___builtin_nop : ident := 50%positive.
+Definition ___builtin_read16_reversed : ident := 46%positive.
+Definition ___builtin_read32_reversed : ident := 47%positive.
+Definition ___builtin_va_arg : ident := 11%positive.
+Definition ___builtin_va_copy : ident := 12%positive.
+Definition ___builtin_va_end : ident := 13%positive.
+Definition ___builtin_va_start : ident := 10%positive.
+Definition ___builtin_write16_reversed : ident := 48%positive.
+Definition ___builtin_write32_reversed : ident := 49%positive.
+Definition ___compcert_i64_dtos : ident := 18%positive.
+Definition ___compcert_i64_dtou : ident := 19%positive.
+Definition ___compcert_i64_sar : ident := 30%positive.
+Definition ___compcert_i64_sdiv : ident := 24%positive.
+Definition ___compcert_i64_shl : ident := 28%positive.
+Definition ___compcert_i64_shr : ident := 29%positive.
+Definition ___compcert_i64_smod : ident := 26%positive.
+Definition ___compcert_i64_smulh : ident := 31%positive.
+Definition ___compcert_i64_stod : ident := 20%positive.
+Definition ___compcert_i64_stof : ident := 22%positive.
+Definition ___compcert_i64_udiv : ident := 25%positive.
+Definition ___compcert_i64_umod : ident := 27%positive.
+Definition ___compcert_i64_umulh : ident := 32%positive.
+Definition ___compcert_i64_utod : ident := 21%positive.
+Definition ___compcert_i64_utof : ident := 23%positive.
+Definition ___compcert_va_composite : ident := 17%positive.
+Definition ___compcert_va_float64 : ident := 16%positive.
+Definition ___compcert_va_int32 : ident := 14%positive.
+Definition ___compcert_va_int64 : ident := 15%positive.
+Definition ___stringlit_1 : ident := 67%positive.
+Definition ___stringlit_2 : ident := 68%positive.
+Definition ___stringlit_3 : ident := 69%positive.
+Definition ___stringlit_4 : ident := 70%positive.
+Definition ___stringlit_5 : ident := 76%positive.
+Definition _argc : ident := 80%positive.
+Definition _argv : ident := 81%positive.
+Definition _curr : ident := 72%positive.
+Definition _dijkstra : ident := 79%positive.
+Definition _dist : ident := 75%positive.
+Definition _getPaths : ident := 77%positive.
+Definition _graph : ident := 62%positive.
+Definition _i : ident := 59%positive.
+Definition _j : ident := 63%positive.
+Definition _main : ident := 82%positive.
+Definition _minVertex : ident := 58%positive.
+Definition _minWeight : ident := 57%positive.
+Definition _popMin : ident := 60%positive.
+Definition _pq : ident := 56%positive.
+Definition _pq_not_emp : ident := 61%positive.
+Definition _prev : ident := 73%positive.
+Definition _printPath : ident := 74%positive.
+Definition _print_graph : ident := 71%positive.
+Definition _printf : ident := 54%positive.
+Definition _rand : ident := 52%positive.
+Definition _random : ident := 64%positive.
+Definition _setup : ident := 65%positive.
+Definition _srand : ident := 53%positive.
+Definition _src : ident := 66%positive.
+Definition _time : ident := 55%positive.
+Definition _u : ident := 78%positive.
+Definition _t'1 : ident := 83%positive.
+Definition _t'2 : ident := 84%positive.
+Definition _t'3 : ident := 85%positive.
+Definition _t'4 : ident := 86%positive.
+Definition _t'5 : ident := 87%positive.
+Definition _t'6 : ident := 88%positive.
+Definition _t'7 : ident := 89%positive.
+Definition _t'8 : ident := 90%positive.
+Definition _t'9 : ident := 91%positive.
 
-Definition v___stringlit_1 := {|
-  gvar_info := (tarray tschar 28);
-  gvar_init := (Init_int8 (Int.repr 65) :: Init_int8 (Int.repr 32) ::
-                Init_int8 (Int.repr 98) :: Init_int8 (Int.repr 108) ::
-                Init_int8 (Int.repr 97) :: Init_int8 (Int.repr 110) ::
-                Init_int8 (Int.repr 107) :: Init_int8 (Int.repr 32) ::
-                Init_int8 (Int.repr 108) :: Init_int8 (Int.repr 105) ::
-                Init_int8 (Int.repr 115) :: Init_int8 (Int.repr 116) ::
-                Init_int8 (Int.repr 32) :: Init_int8 (Int.repr 119) ::
-                Init_int8 (Int.repr 97) :: Init_int8 (Int.repr 115) ::
-                Init_int8 (Int.repr 32) :: Init_int8 (Int.repr 112) ::
-                Init_int8 (Int.repr 114) :: Init_int8 (Int.repr 111) ::
-                Init_int8 (Int.repr 118) :: Init_int8 (Int.repr 105) ::
-                Init_int8 (Int.repr 100) :: Init_int8 (Int.repr 101) ::
-                Init_int8 (Int.repr 100) :: Init_int8 (Int.repr 46) ::
-                Init_int8 (Int.repr 10) :: Init_int8 (Int.repr 0) :: nil);
-  gvar_readonly := true;
-  gvar_volatile := false
-|}.
-
-Definition v___stringlit_6 := {|
+Definition v___stringlit_4 := {|
   gvar_info := (tarray tschar 13);
   gvar_init := (Init_int8 (Int.repr 83) :: Init_int8 (Int.repr 111) ::
                 Init_int8 (Int.repr 117) :: Init_int8 (Int.repr 114) ::
@@ -167,61 +120,33 @@ Definition v___stringlit_6 := {|
   gvar_volatile := false
 |}.
 
-Definition v___stringlit_7 := {|
-  gvar_info := (tarray tschar 45);
-  gvar_init := (Init_int8 (Int.repr 73) :: Init_int8 (Int.repr 109) ::
-                Init_int8 (Int.repr 112) :: Init_int8 (Int.repr 114) ::
-                Init_int8 (Int.repr 111) :: Init_int8 (Int.repr 118) ::
-                Init_int8 (Int.repr 101) :: Init_int8 (Int.repr 100) ::
-                Init_int8 (Int.repr 32) :: Init_int8 (Int.repr 116) ::
-                Init_int8 (Int.repr 104) :: Init_int8 (Int.repr 101) ::
-                Init_int8 (Int.repr 32) :: Init_int8 (Int.repr 100) ::
-                Init_int8 (Int.repr 105) :: Init_int8 (Int.repr 115) ::
-                Init_int8 (Int.repr 116) :: Init_int8 (Int.repr 32) ::
-                Init_int8 (Int.repr 116) :: Init_int8 (Int.repr 111) ::
-                Init_int8 (Int.repr 32) :: Init_int8 (Int.repr 103) ::
-                Init_int8 (Int.repr 101) :: Init_int8 (Int.repr 116) ::
-                Init_int8 (Int.repr 32) :: Init_int8 (Int.repr 116) ::
-                Init_int8 (Int.repr 111) :: Init_int8 (Int.repr 32) ::
+Definition v___stringlit_5 := {|
+  gvar_info := (tarray tschar 39);
+  gvar_init := (Init_int8 (Int.repr 10) :: Init_int8 (Int.repr 84) ::
+                Init_int8 (Int.repr 114) :: Init_int8 (Int.repr 97) ::
                 Init_int8 (Int.repr 118) :: Init_int8 (Int.repr 101) ::
-                Init_int8 (Int.repr 114) :: Init_int8 (Int.repr 116) ::
-                Init_int8 (Int.repr 101) :: Init_int8 (Int.repr 120) ::
+                Init_int8 (Int.repr 108) :: Init_int8 (Int.repr 32) ::
+                Init_int8 (Int.repr 102) :: Init_int8 (Int.repr 114) ::
+                Init_int8 (Int.repr 111) :: Init_int8 (Int.repr 109) ::
                 Init_int8 (Int.repr 32) :: Init_int8 (Int.repr 37) ::
                 Init_int8 (Int.repr 100) :: Init_int8 (Int.repr 32) ::
                 Init_int8 (Int.repr 116) :: Init_int8 (Int.repr 111) ::
                 Init_int8 (Int.repr 32) :: Init_int8 (Int.repr 37) ::
-                Init_int8 (Int.repr 100) :: Init_int8 (Int.repr 10) ::
+                Init_int8 (Int.repr 100) :: Init_int8 (Int.repr 32) ::
+                Init_int8 (Int.repr 97) :: Init_int8 (Int.repr 116) ::
+                Init_int8 (Int.repr 32) :: Init_int8 (Int.repr 99) ::
+                Init_int8 (Int.repr 111) :: Init_int8 (Int.repr 115) ::
+                Init_int8 (Int.repr 116) :: Init_int8 (Int.repr 32) ::
+                Init_int8 (Int.repr 37) :: Init_int8 (Int.repr 100) ::
+                Init_int8 (Int.repr 32) :: Init_int8 (Int.repr 118) ::
+                Init_int8 (Int.repr 105) :: Init_int8 (Int.repr 97) ::
+                Init_int8 (Int.repr 58) :: Init_int8 (Int.repr 32) ::
                 Init_int8 (Int.repr 0) :: nil);
   gvar_readonly := true;
   gvar_volatile := false
 |}.
 
-Definition v___stringlit_9 := {|
-  gvar_info := (tarray tschar 38);
-  gvar_init := (Init_int8 (Int.repr 86) :: Init_int8 (Int.repr 101) ::
-                Init_int8 (Int.repr 114) :: Init_int8 (Int.repr 116) ::
-                Init_int8 (Int.repr 101) :: Init_int8 (Int.repr 120) ::
-                Init_int8 (Int.repr 32) :: Init_int8 (Int.repr 37) ::
-                Init_int8 (Int.repr 100) :: Init_int8 (Int.repr 32) ::
-                Init_int8 (Int.repr 119) :: Init_int8 (Int.repr 97) ::
-                Init_int8 (Int.repr 115) :: Init_int8 (Int.repr 32) ::
-                Init_int8 (Int.repr 117) :: Init_int8 (Int.repr 110) ::
-                Init_int8 (Int.repr 114) :: Init_int8 (Int.repr 101) ::
-                Init_int8 (Int.repr 97) :: Init_int8 (Int.repr 99) ::
-                Init_int8 (Int.repr 104) :: Init_int8 (Int.repr 97) ::
-                Init_int8 (Int.repr 98) :: Init_int8 (Int.repr 108) ::
-                Init_int8 (Int.repr 101) :: Init_int8 (Int.repr 32) ::
-                Init_int8 (Int.repr 97) :: Init_int8 (Int.repr 108) ::
-                Init_int8 (Int.repr 116) :: Init_int8 (Int.repr 111) ::
-                Init_int8 (Int.repr 103) :: Init_int8 (Int.repr 101) ::
-                Init_int8 (Int.repr 116) :: Init_int8 (Int.repr 104) ::
-                Init_int8 (Int.repr 101) :: Init_int8 (Int.repr 114) ::
-                Init_int8 (Int.repr 10) :: Init_int8 (Int.repr 0) :: nil);
-  gvar_readonly := true;
-  gvar_volatile := false
-|}.
-
-Definition v___stringlit_2 := {|
+Definition v___stringlit_1 := {|
   gvar_info := (tarray tschar 4);
   gvar_init := (Init_int8 (Int.repr 37) :: Init_int8 (Int.repr 100) ::
                 Init_int8 (Int.repr 9) :: Init_int8 (Int.repr 0) :: nil);
@@ -236,18 +161,7 @@ Definition v___stringlit_3 := {|
   gvar_volatile := false
 |}.
 
-Definition v___stringlit_4 := {|
-  gvar_info := (tarray tschar 10);
-  gvar_init := (Init_int8 (Int.repr 40) :: Init_int8 (Int.repr 37) ::
-                Init_int8 (Int.repr 100) :: Init_int8 (Int.repr 44) ::
-                Init_int8 (Int.repr 32) :: Init_int8 (Int.repr 37) ::
-                Init_int8 (Int.repr 100) :: Init_int8 (Int.repr 41) ::
-                Init_int8 (Int.repr 9) :: Init_int8 (Int.repr 0) :: nil);
-  gvar_readonly := true;
-  gvar_volatile := false
-|}.
-
-Definition v___stringlit_5 := {|
+Definition v___stringlit_2 := {|
   gvar_info := (tarray tschar 3);
   gvar_init := (Init_int8 (Int.repr 45) :: Init_int8 (Int.repr 9) ::
                 Init_int8 (Int.repr 0) :: nil);
@@ -255,441 +169,93 @@ Definition v___stringlit_5 := {|
   gvar_volatile := false
 |}.
 
-Definition v___stringlit_8 := {|
-  gvar_info := (tarray tschar 38);
-  gvar_init := (Init_int8 (Int.repr 84) :: Init_int8 (Int.repr 114) ::
-                Init_int8 (Int.repr 97) :: Init_int8 (Int.repr 118) ::
-                Init_int8 (Int.repr 101) :: Init_int8 (Int.repr 108) ::
-                Init_int8 (Int.repr 32) :: Init_int8 (Int.repr 102) ::
-                Init_int8 (Int.repr 114) :: Init_int8 (Int.repr 111) ::
-                Init_int8 (Int.repr 109) :: Init_int8 (Int.repr 32) ::
-                Init_int8 (Int.repr 37) :: Init_int8 (Int.repr 100) ::
-                Init_int8 (Int.repr 32) :: Init_int8 (Int.repr 116) ::
-                Init_int8 (Int.repr 111) :: Init_int8 (Int.repr 32) ::
-                Init_int8 (Int.repr 37) :: Init_int8 (Int.repr 100) ::
-                Init_int8 (Int.repr 32) :: Init_int8 (Int.repr 97) ::
-                Init_int8 (Int.repr 116) :: Init_int8 (Int.repr 32) ::
-                Init_int8 (Int.repr 99) :: Init_int8 (Int.repr 111) ::
-                Init_int8 (Int.repr 115) :: Init_int8 (Int.repr 116) ::
-                Init_int8 (Int.repr 32) :: Init_int8 (Int.repr 37) ::
-                Init_int8 (Int.repr 100) :: Init_int8 (Int.repr 32) ::
-                Init_int8 (Int.repr 118) :: Init_int8 (Int.repr 105) ::
-                Init_int8 (Int.repr 97) :: Init_int8 (Int.repr 58) ::
-                Init_int8 (Int.repr 32) :: Init_int8 (Int.repr 0) :: nil);
-  gvar_readonly := true;
-  gvar_volatile := false
-|}.
-
-Definition f_push := {|
-  fn_return := tvoid;
-  fn_callconv := cc_default;
-  fn_params := ((_vertex, tint) :: (_weight, tint) ::
-                (_list, (tptr (tptr (Tstruct _Node noattr)))) :: nil);
-  fn_vars := nil;
-  fn_temps := ((_newHead, (tptr (Tstruct _Node noattr))) ::
-               (_t'1, (tptr tvoid)) ::
-               (_t'4, (tptr (Tstruct _Node noattr))) ::
-               (_t'3, (tptr (Tstruct _Node noattr))) ::
-               (_t'2, (tptr (Tstruct _Node noattr))) :: nil);
-  fn_body :=
-(Ssequence
-  (Ssequence
-    (Scall (Some _t'1)
-      (Evar _malloc (Tfunction (Tcons tuint Tnil) (tptr tvoid) cc_default))
-      ((Esizeof (Tstruct _Node noattr) tuint) :: nil))
-    (Sset _newHead
-      (Ecast (Etempvar _t'1 (tptr tvoid)) (tptr (Tstruct _Node noattr)))))
-  (Ssequence
-    (Sassign
-      (Efield
-        (Ederef (Etempvar _newHead (tptr (Tstruct _Node noattr)))
-          (Tstruct _Node noattr)) _vertex tint) (Etempvar _vertex tint))
-    (Ssequence
-      (Sassign
-        (Efield
-          (Ederef (Etempvar _newHead (tptr (Tstruct _Node noattr)))
-            (Tstruct _Node noattr)) _weight tint) (Etempvar _weight tint))
-      (Ssequence
-        (Sassign
-          (Efield
-            (Ederef (Etempvar _newHead (tptr (Tstruct _Node noattr)))
-              (Tstruct _Node noattr)) _prev (tptr (Tstruct _Node noattr)))
-          (Ecast (Econst_int (Int.repr 0) tint) (tptr tvoid)))
-        (Ssequence
-          (Ssequence
-            (Sset _t'4
-              (Ederef (Etempvar _list (tptr (tptr (Tstruct _Node noattr))))
-                (tptr (Tstruct _Node noattr))))
-            (Sassign
-              (Efield
-                (Ederef (Etempvar _newHead (tptr (Tstruct _Node noattr)))
-                  (Tstruct _Node noattr)) _next
-                (tptr (Tstruct _Node noattr)))
-              (Etempvar _t'4 (tptr (Tstruct _Node noattr)))))
-          (Ssequence
-            (Ssequence
-              (Sset _t'2
-                (Ederef (Etempvar _list (tptr (tptr (Tstruct _Node noattr))))
-                  (tptr (Tstruct _Node noattr))))
-              (Sifthenelse (Ebinop One
-                             (Etempvar _t'2 (tptr (Tstruct _Node noattr)))
-                             (Ecast (Econst_int (Int.repr 0) tint)
-                               (tptr tvoid)) tint)
-                (Ssequence
-                  (Sset _t'3
-                    (Ederef
-                      (Etempvar _list (tptr (tptr (Tstruct _Node noattr))))
-                      (tptr (Tstruct _Node noattr))))
-                  (Sassign
-                    (Efield
-                      (Ederef (Etempvar _t'3 (tptr (Tstruct _Node noattr)))
-                        (Tstruct _Node noattr)) _prev
-                      (tptr (Tstruct _Node noattr)))
-                    (Etempvar _newHead (tptr (Tstruct _Node noattr)))))
-                Sskip))
-            (Sassign
-              (Ederef (Etempvar _list (tptr (tptr (Tstruct _Node noattr))))
-                (tptr (Tstruct _Node noattr)))
-              (Etempvar _newHead (tptr (Tstruct _Node noattr))))))))))
-|}.
-
-Definition f_deleteNode := {|
-  fn_return := tvoid;
-  fn_callconv := cc_default;
-  fn_params := ((_del, (tptr (Tstruct _Node noattr))) ::
-                (_head, (tptr (tptr (Tstruct _Node noattr)))) :: nil);
-  fn_vars := nil;
-  fn_temps := ((_t'1, tint) :: (_t'10, (tptr (Tstruct _Node noattr))) ::
-               (_t'9, (tptr (Tstruct _Node noattr))) ::
-               (_t'8, (tptr (Tstruct _Node noattr))) ::
-               (_t'7, (tptr (Tstruct _Node noattr))) ::
-               (_t'6, (tptr (Tstruct _Node noattr))) ::
-               (_t'5, (tptr (Tstruct _Node noattr))) ::
-               (_t'4, (tptr (Tstruct _Node noattr))) ::
-               (_t'3, (tptr (Tstruct _Node noattr))) ::
-               (_t'2, (tptr (Tstruct _Node noattr))) :: nil);
-  fn_body :=
-(Ssequence
-  (Ssequence
-    (Ssequence
-      (Sset _t'10
-        (Ederef (Etempvar _head (tptr (tptr (Tstruct _Node noattr))))
-          (tptr (Tstruct _Node noattr))))
-      (Sifthenelse (Ebinop Oeq (Etempvar _t'10 (tptr (Tstruct _Node noattr)))
-                     (Ecast (Econst_int (Int.repr 0) tint) (tptr tvoid))
-                     tint)
-        (Sset _t'1 (Econst_int (Int.repr 1) tint))
-        (Sset _t'1
-          (Ecast
-            (Ebinop Oeq (Etempvar _del (tptr (Tstruct _Node noattr)))
-              (Ecast (Econst_int (Int.repr 0) tint) (tptr tvoid)) tint)
-            tbool))))
-    (Sifthenelse (Etempvar _t'1 tint) (Sreturn None) Sskip))
-  (Ssequence
-    (Ssequence
-      (Sset _t'8
-        (Ederef (Etempvar _head (tptr (tptr (Tstruct _Node noattr))))
-          (tptr (Tstruct _Node noattr))))
-      (Sifthenelse (Ebinop Oeq (Etempvar _t'8 (tptr (Tstruct _Node noattr)))
-                     (Etempvar _del (tptr (Tstruct _Node noattr))) tint)
-        (Ssequence
-          (Sset _t'9
-            (Efield
-              (Ederef (Etempvar _del (tptr (Tstruct _Node noattr)))
-                (Tstruct _Node noattr)) _next (tptr (Tstruct _Node noattr))))
-          (Sassign
-            (Ederef (Etempvar _head (tptr (tptr (Tstruct _Node noattr))))
-              (tptr (Tstruct _Node noattr)))
-            (Etempvar _t'9 (tptr (Tstruct _Node noattr)))))
-        Sskip))
-    (Ssequence
-      (Ssequence
-        (Sset _t'5
-          (Efield
-            (Ederef (Etempvar _del (tptr (Tstruct _Node noattr)))
-              (Tstruct _Node noattr)) _next (tptr (Tstruct _Node noattr))))
-        (Sifthenelse (Ebinop One
-                       (Etempvar _t'5 (tptr (Tstruct _Node noattr)))
-                       (Ecast (Econst_int (Int.repr 0) tint) (tptr tvoid))
-                       tint)
-          (Ssequence
-            (Sset _t'6
-              (Efield
-                (Ederef (Etempvar _del (tptr (Tstruct _Node noattr)))
-                  (Tstruct _Node noattr)) _next
-                (tptr (Tstruct _Node noattr))))
-            (Ssequence
-              (Sset _t'7
-                (Efield
-                  (Ederef (Etempvar _del (tptr (Tstruct _Node noattr)))
-                    (Tstruct _Node noattr)) _prev
-                  (tptr (Tstruct _Node noattr))))
-              (Sassign
-                (Efield
-                  (Ederef (Etempvar _t'6 (tptr (Tstruct _Node noattr)))
-                    (Tstruct _Node noattr)) _prev
-                  (tptr (Tstruct _Node noattr)))
-                (Etempvar _t'7 (tptr (Tstruct _Node noattr))))))
-          Sskip))
-      (Ssequence
-        (Ssequence
-          (Sset _t'2
-            (Efield
-              (Ederef (Etempvar _del (tptr (Tstruct _Node noattr)))
-                (Tstruct _Node noattr)) _prev (tptr (Tstruct _Node noattr))))
-          (Sifthenelse (Ebinop One
-                         (Etempvar _t'2 (tptr (Tstruct _Node noattr)))
-                         (Ecast (Econst_int (Int.repr 0) tint) (tptr tvoid))
-                         tint)
-            (Ssequence
-              (Sset _t'3
-                (Efield
-                  (Ederef (Etempvar _del (tptr (Tstruct _Node noattr)))
-                    (Tstruct _Node noattr)) _prev
-                  (tptr (Tstruct _Node noattr))))
-              (Ssequence
-                (Sset _t'4
-                  (Efield
-                    (Ederef (Etempvar _del (tptr (Tstruct _Node noattr)))
-                      (Tstruct _Node noattr)) _next
-                    (tptr (Tstruct _Node noattr))))
-                (Sassign
-                  (Efield
-                    (Ederef (Etempvar _t'3 (tptr (Tstruct _Node noattr)))
-                      (Tstruct _Node noattr)) _next
-                    (tptr (Tstruct _Node noattr)))
-                  (Etempvar _t'4 (tptr (Tstruct _Node noattr))))))
-            Sskip))
-        (Ssequence
-          (Scall None
-            (Evar _free (Tfunction (Tcons (tptr tvoid) Tnil) tvoid
-                          cc_default))
-            ((Etempvar _del (tptr (Tstruct _Node noattr))) :: nil))
-          (Sreturn None))))))
-|}.
-
 Definition f_popMin := {|
   fn_return := tint;
   fn_callconv := cc_default;
-  fn_params := ((_head, (tptr (tptr (Tstruct _Node noattr)))) :: nil);
+  fn_params := ((_pq, (tptr tint)) :: nil);
   fn_vars := nil;
-  fn_temps := ((_minWeight, tint) :: (_minVertex, tint) ::
-               (_minNode, (tptr (Tstruct _Node noattr))) ::
-               (_current, (tptr (Tstruct _Node noattr))) :: (_t'1, tint) ::
-               nil);
+  fn_temps := ((_minWeight, tint) :: (_minVertex, tint) :: (_i, tint) ::
+               (_t'1, tint) :: nil);
   fn_body :=
 (Ssequence
   (Sset _minWeight (Econst_int (Int.repr 2147483647) tint))
   (Ssequence
     (Sset _minVertex (Eunop Oneg (Econst_int (Int.repr 1) tint) tint))
     (Ssequence
-      (Sset _minNode (Ecast (Econst_int (Int.repr 0) tint) (tptr tvoid)))
       (Ssequence
-        (Sset _current
-          (Ederef (Etempvar _head (tptr (tptr (Tstruct _Node noattr))))
-            (tptr (Tstruct _Node noattr))))
-        (Ssequence
-          (Swhile
-            (Ebinop One (Etempvar _current (tptr (Tstruct _Node noattr)))
-              (Ecast (Econst_int (Int.repr 0) tint) (tptr tvoid)) tint)
-            (Ssequence
-              (Ssequence
-                (Sset _t'1
-                  (Efield
-                    (Ederef (Etempvar _current (tptr (Tstruct _Node noattr)))
-                      (Tstruct _Node noattr)) _weight tint))
-                (Sifthenelse (Ebinop Olt (Etempvar _t'1 tint)
-                               (Etempvar _minWeight tint) tint)
-                  (Ssequence
-                    (Sset _minWeight
-                      (Efield
-                        (Ederef
-                          (Etempvar _current (tptr (Tstruct _Node noattr)))
-                          (Tstruct _Node noattr)) _weight tint))
-                    (Ssequence
-                      (Sset _minVertex
-                        (Efield
-                          (Ederef
-                            (Etempvar _current (tptr (Tstruct _Node noattr)))
-                            (Tstruct _Node noattr)) _vertex tint))
-                      (Sset _minNode
-                        (Etempvar _current (tptr (Tstruct _Node noattr))))))
-                  Sskip))
-              (Sset _current
-                (Efield
-                  (Ederef (Etempvar _current (tptr (Tstruct _Node noattr)))
-                    (Tstruct _Node noattr)) _next
-                  (tptr (Tstruct _Node noattr))))))
+        (Sset _i (Econst_int (Int.repr 0) tint))
+        (Sloop
           (Ssequence
-            (Scall None
-              (Evar _deleteNode (Tfunction
-                                  (Tcons (tptr (Tstruct _Node noattr))
-                                    (Tcons
-                                      (tptr (tptr (Tstruct _Node noattr)))
-                                      Tnil)) tvoid cc_default))
-              ((Etempvar _minNode (tptr (Tstruct _Node noattr))) ::
-               (Etempvar _head (tptr (tptr (Tstruct _Node noattr)))) :: nil))
-            (Sreturn (Some (Etempvar _minVertex tint)))))))))
-|}.
-
-Definition f_adjustWeight := {|
-  fn_return := tvoid;
-  fn_callconv := cc_default;
-  fn_params := ((_vertex, tint) :: (_newWeight, tint) ::
-                (_head, (tptr (tptr (Tstruct _Node noattr)))) :: nil);
-  fn_vars := nil;
-  fn_temps := ((_current, (tptr (Tstruct _Node noattr))) :: (_t'1, tint) ::
-               nil);
-  fn_body :=
-(Ssequence
-  (Sset _current
-    (Ederef (Etempvar _head (tptr (tptr (Tstruct _Node noattr))))
-      (tptr (Tstruct _Node noattr))))
-  (Swhile
-    (Ebinop One (Etempvar _current (tptr (Tstruct _Node noattr)))
-      (Ecast (Econst_int (Int.repr 0) tint) (tptr tvoid)) tint)
-    (Ssequence
+            (Sifthenelse (Ebinop Olt (Etempvar _i tint)
+                           (Econst_int (Int.repr 8) tint) tint)
+              Sskip
+              Sbreak)
+            (Ssequence
+              (Sset _t'1
+                (Ederef
+                  (Ebinop Oadd (Etempvar _pq (tptr tint)) (Etempvar _i tint)
+                    (tptr tint)) tint))
+              (Sifthenelse (Ebinop Olt (Etempvar _t'1 tint)
+                             (Etempvar _minWeight tint) tint)
+                (Ssequence
+                  (Sset _minVertex (Etempvar _i tint))
+                  (Sset _minWeight
+                    (Ederef
+                      (Ebinop Oadd (Etempvar _pq (tptr tint))
+                        (Etempvar _i tint) (tptr tint)) tint)))
+                Sskip)))
+          (Sset _i
+            (Ebinop Oadd (Etempvar _i tint) (Econst_int (Int.repr 1) tint)
+              tint))))
       (Ssequence
-        (Sset _t'1
-          (Efield
-            (Ederef (Etempvar _current (tptr (Tstruct _Node noattr)))
-              (Tstruct _Node noattr)) _vertex tint))
-        (Sifthenelse (Ebinop Oeq (Etempvar _t'1 tint) (Etempvar _vertex tint)
-                       tint)
-          (Ssequence
-            (Sassign
-              (Efield
-                (Ederef (Etempvar _current (tptr (Tstruct _Node noattr)))
-                  (Tstruct _Node noattr)) _weight tint)
-              (Etempvar _newWeight tint))
-            (Sreturn None))
-          Sskip))
-      (Sset _current
-        (Efield
-          (Ederef (Etempvar _current (tptr (Tstruct _Node noattr)))
-            (Tstruct _Node noattr)) _next (tptr (Tstruct _Node noattr)))))))
+        (Sifthenelse (Ebinop One (Etempvar _minVertex tint)
+                       (Eunop Oneg (Econst_int (Int.repr 1) tint) tint) tint)
+          (Sassign
+            (Ederef
+              (Ebinop Oadd (Etempvar _pq (tptr tint))
+                (Etempvar _minVertex tint) (tptr tint)) tint)
+            (Econst_int (Int.repr 2147483647) tint))
+          Sskip)
+        (Sreturn (Some (Etempvar _minVertex tint)))))))
 |}.
 
-Definition f_print_verts := {|
-  fn_return := tvoid;
+Definition f_pq_not_emp := {|
+  fn_return := tint;
   fn_callconv := cc_default;
-  fn_params := ((_list, (tptr (Tstruct _Node noattr))) :: nil);
+  fn_params := ((_pq, (tptr tint)) :: nil);
   fn_vars := nil;
-  fn_temps := ((_current, (tptr (Tstruct _Node noattr))) :: (_t'1, tint) ::
-               nil);
+  fn_temps := ((_i, tint) :: (_t'1, tint) :: nil);
   fn_body :=
 (Ssequence
-  (Sifthenelse (Ebinop Oeq (Etempvar _list (tptr (Tstruct _Node noattr)))
-                 (Ecast (Econst_int (Int.repr 0) tint) (tptr tvoid)) tint)
-    (Scall None
-      (Evar _printf (Tfunction (Tcons (tptr tschar) Tnil) tint
-                      {|cc_vararg:=true; cc_unproto:=false; cc_structret:=false|}))
-      ((Evar ___stringlit_1 (tarray tschar 28)) :: nil))
-    Sskip)
   (Ssequence
-    (Sset _current (Etempvar _list (tptr (Tstruct _Node noattr))))
-    (Ssequence
-      (Swhile
-        (Ebinop One (Etempvar _current (tptr (Tstruct _Node noattr)))
-          (Ecast (Econst_int (Int.repr 0) tint) (tptr tvoid)) tint)
+    (Sset _i (Econst_int (Int.repr 0) tint))
+    (Sloop
+      (Ssequence
+        (Sifthenelse (Ebinop Olt (Etempvar _i tint)
+                       (Econst_int (Int.repr 8) tint) tint)
+          Sskip
+          Sbreak)
         (Ssequence
-          (Ssequence
-            (Sset _t'1
-              (Efield
-                (Ederef (Etempvar _current (tptr (Tstruct _Node noattr)))
-                  (Tstruct _Node noattr)) _vertex tint))
-            (Scall None
-              (Evar _printf (Tfunction (Tcons (tptr tschar) Tnil) tint
-                              {|cc_vararg:=true; cc_unproto:=false; cc_structret:=false|}))
-              ((Evar ___stringlit_2 (tarray tschar 4)) ::
-               (Etempvar _t'1 tint) :: nil)))
-          (Sset _current
-            (Efield
-              (Ederef (Etempvar _current (tptr (Tstruct _Node noattr)))
-                (Tstruct _Node noattr)) _next (tptr (Tstruct _Node noattr))))))
-      (Scall None
-        (Evar _printf (Tfunction (Tcons (tptr tschar) Tnil) tint
-                        {|cc_vararg:=true; cc_unproto:=false; cc_structret:=false|}))
-        ((Evar ___stringlit_3 (tarray tschar 2)) :: nil)))))
-|}.
-
-Definition f_print_list := {|
-  fn_return := tvoid;
-  fn_callconv := cc_default;
-  fn_params := ((_list, (tptr (Tstruct _Node noattr))) :: nil);
-  fn_vars := nil;
-  fn_temps := ((_current, (tptr (Tstruct _Node noattr))) :: (_t'2, tint) ::
-               (_t'1, tint) :: nil);
-  fn_body :=
-(Ssequence
-  (Sifthenelse (Ebinop Oeq (Etempvar _list (tptr (Tstruct _Node noattr)))
-                 (Ecast (Econst_int (Int.repr 0) tint) (tptr tvoid)) tint)
-    (Scall None
-      (Evar _printf (Tfunction (Tcons (tptr tschar) Tnil) tint
-                      {|cc_vararg:=true; cc_unproto:=false; cc_structret:=false|}))
-      ((Evar ___stringlit_1 (tarray tschar 28)) :: nil))
-    Sskip)
-  (Ssequence
-    (Sset _current (Etempvar _list (tptr (Tstruct _Node noattr))))
-    (Ssequence
-      (Swhile
-        (Ebinop One (Etempvar _current (tptr (Tstruct _Node noattr)))
-          (Ecast (Econst_int (Int.repr 0) tint) (tptr tvoid)) tint)
-        (Ssequence
-          (Ssequence
-            (Sset _t'1
-              (Efield
-                (Ederef (Etempvar _current (tptr (Tstruct _Node noattr)))
-                  (Tstruct _Node noattr)) _vertex tint))
-            (Ssequence
-              (Sset _t'2
-                (Efield
-                  (Ederef (Etempvar _current (tptr (Tstruct _Node noattr)))
-                    (Tstruct _Node noattr)) _weight tint))
-              (Scall None
-                (Evar _printf (Tfunction (Tcons (tptr tschar) Tnil) tint
-                                {|cc_vararg:=true; cc_unproto:=false; cc_structret:=false|}))
-                ((Evar ___stringlit_4 (tarray tschar 10)) ::
-                 (Etempvar _t'1 tint) :: (Etempvar _t'2 tint) :: nil))))
-          (Sset _current
-            (Efield
-              (Ederef (Etempvar _current (tptr (Tstruct _Node noattr)))
-                (Tstruct _Node noattr)) _next (tptr (Tstruct _Node noattr))))))
-      (Scall None
-        (Evar _printf (Tfunction (Tcons (tptr tschar) Tnil) tint
-                        {|cc_vararg:=true; cc_unproto:=false; cc_structret:=false|}))
-        ((Evar ___stringlit_3 (tarray tschar 2)) :: nil)))))
-|}.
-
-Definition v_graph := {|
-  gvar_info := (tarray (tarray tint 8) 8);
-  gvar_init := (Init_space 256 :: nil);
-  gvar_readonly := false;
-  gvar_volatile := false
-|}.
-
-Definition v_src := {|
-  gvar_info := tint;
-  gvar_init := (Init_space 4 :: nil);
-  gvar_readonly := false;
-  gvar_volatile := false
-|}.
-
-Definition v_dst := {|
-  gvar_info := tint;
-  gvar_init := (Init_space 4 :: nil);
-  gvar_readonly := false;
-  gvar_volatile := false
+          (Sset _t'1
+            (Ederef
+              (Ebinop Oadd (Etempvar _pq (tptr tint)) (Etempvar _i tint)
+                (tptr tint)) tint))
+          (Sifthenelse (Ebinop Olt (Etempvar _t'1 tint)
+                         (Econst_int (Int.repr 2147483647) tint) tint)
+            (Sreturn (Some (Econst_int (Int.repr 1) tint)))
+            Sskip)))
+      (Sset _i
+        (Ebinop Oadd (Etempvar _i tint) (Econst_int (Int.repr 1) tint) tint))))
+  (Sreturn (Some (Econst_int (Int.repr 0) tint))))
 |}.
 
 Definition f_setup := {|
   fn_return := tvoid;
   fn_callconv := cc_default;
-  fn_params := nil;
+  fn_params := ((_graph, (tptr (tarray tint 8))) :: nil);
   fn_vars := nil;
-  fn_temps := ((_i, tint) :: (_j, tint) :: (_random, tint) :: (_t'5, tint) ::
-               (_t'4, tint) :: (_t'3, tint) :: (_t'2, tint) ::
-               (_t'1, tint) :: nil);
+  fn_temps := ((_i, tint) :: (_j, tint) :: (_random, tint) :: (_t'4, tint) ::
+               (_t'3, tint) :: (_t'2, tint) :: (_t'1, tint) :: nil);
   fn_body :=
 (Ssequence
   (Ssequence
@@ -699,76 +265,69 @@ Definition f_setup := {|
     (Scall None (Evar _srand (Tfunction (Tcons tuint Tnil) tvoid cc_default))
       ((Ecast (Etempvar _t'1 tint) tuint) :: nil)))
   (Ssequence
-    (Ssequence
-      (Scall (Some _t'2) (Evar _rand (Tfunction Tnil tint cc_default)) nil)
-      (Sassign (Evar _src tint)
-        (Ebinop Omod (Etempvar _t'2 tint) (Econst_int (Int.repr 8) tint)
-          tint)))
-    (Ssequence
-      (Sset _i (Econst_int (Int.repr 0) tint))
-      (Sloop
+    (Sset _i (Econst_int (Int.repr 0) tint))
+    (Sloop
+      (Ssequence
+        (Sifthenelse (Ebinop Olt (Etempvar _i tint)
+                       (Econst_int (Int.repr 8) tint) tint)
+          Sskip
+          Sbreak)
         (Ssequence
-          (Sifthenelse (Ebinop Olt (Etempvar _i tint)
-                         (Econst_int (Int.repr 8) tint) tint)
-            Sskip
-            Sbreak)
-          (Ssequence
-            (Sset _j (Econst_int (Int.repr 0) tint))
-            (Sloop
+          (Sset _j (Econst_int (Int.repr 0) tint))
+          (Sloop
+            (Ssequence
+              (Sifthenelse (Ebinop Ole (Etempvar _j tint)
+                             (Econst_int (Int.repr 8) tint) tint)
+                Sskip
+                Sbreak)
               (Ssequence
-                (Sifthenelse (Ebinop Ole (Etempvar _j tint)
-                               (Econst_int (Int.repr 8) tint) tint)
-                  Sskip
-                  Sbreak)
                 (Ssequence
-                  (Ssequence
-                    (Scall (Some _t'3)
-                      (Evar _rand (Tfunction Tnil tint cc_default)) nil)
-                    (Sset _random
-                      (Ebinop Omod (Etempvar _t'3 tint)
-                        (Ebinop Omul (Econst_int (Int.repr 5) tint)
-                          (Econst_int (Int.repr 50) tint) tint) tint)))
-                  (Ssequence
-                    (Sifthenelse (Ebinop Oeq (Etempvar _i tint)
-                                   (Etempvar _j tint) tint)
-                      (Sset _t'4 (Ecast (Econst_int (Int.repr 0) tint) tint))
-                      (Sifthenelse (Ebinop Ogt (Etempvar _random tint)
-                                     (Econst_int (Int.repr 50) tint) tint)
-                        (Ssequence
-                          (Sset _t'5
-                            (Ecast (Econst_int (Int.repr 2147483647) tint)
-                              tint))
-                          (Sset _t'4 (Ecast (Etempvar _t'5 tint) tint)))
-                        (Ssequence
-                          (Sset _t'5
-                            (Ecast
-                              (Ebinop Oadd (Econst_int (Int.repr 1) tint)
-                                (Etempvar _random tint) tint) tint))
-                          (Sset _t'4 (Ecast (Etempvar _t'5 tint) tint)))))
-                    (Sassign
-                      (Ederef
-                        (Ebinop Oadd
-                          (Ederef
-                            (Ebinop Oadd
-                              (Evar _graph (tarray (tarray tint 8) 8))
-                              (Etempvar _i tint) (tptr (tarray tint 8)))
-                            (tarray tint 8)) (Etempvar _j tint) (tptr tint))
-                        tint) (Etempvar _t'4 tint)))))
-              (Sset _j
-                (Ebinop Oadd (Etempvar _j tint)
-                  (Econst_int (Int.repr 1) tint) tint)))))
-        (Sset _i
-          (Ebinop Oadd (Etempvar _i tint) (Econst_int (Int.repr 1) tint)
-            tint))))))
+                  (Scall (Some _t'2)
+                    (Evar _rand (Tfunction Tnil tint cc_default)) nil)
+                  (Sset _random
+                    (Ebinop Omod (Etempvar _t'2 tint)
+                      (Ebinop Omul (Econst_int (Int.repr 3) tint)
+                        (Econst_int (Int.repr 50) tint) tint) tint)))
+                (Ssequence
+                  (Sifthenelse (Ebinop Oeq (Etempvar _i tint)
+                                 (Etempvar _j tint) tint)
+                    (Sset _t'3 (Ecast (Econst_int (Int.repr 0) tint) tint))
+                    (Sifthenelse (Ebinop Ogt (Etempvar _random tint)
+                                   (Econst_int (Int.repr 50) tint) tint)
+                      (Ssequence
+                        (Sset _t'4
+                          (Ecast (Econst_int (Int.repr 2147483647) tint)
+                            tint))
+                        (Sset _t'3 (Ecast (Etempvar _t'4 tint) tint)))
+                      (Ssequence
+                        (Sset _t'4
+                          (Ecast
+                            (Ebinop Oadd (Econst_int (Int.repr 1) tint)
+                              (Etempvar _random tint) tint) tint))
+                        (Sset _t'3 (Ecast (Etempvar _t'4 tint) tint)))))
+                  (Sassign
+                    (Ederef
+                      (Ebinop Oadd
+                        (Ederef
+                          (Ebinop Oadd
+                            (Etempvar _graph (tptr (tarray tint 8)))
+                            (Etempvar _i tint) (tptr (tarray tint 8)))
+                          (tarray tint 8)) (Etempvar _j tint) (tptr tint))
+                      tint) (Etempvar _t'3 tint)))))
+            (Sset _j
+              (Ebinop Oadd (Etempvar _j tint) (Econst_int (Int.repr 1) tint)
+                tint)))))
+      (Sset _i
+        (Ebinop Oadd (Etempvar _i tint) (Econst_int (Int.repr 1) tint) tint)))))
 |}.
 
 Definition f_print_graph := {|
   fn_return := tvoid;
   fn_callconv := cc_default;
-  fn_params := nil;
+  fn_params := ((_graph, (tptr (tarray tint 8))) :: (_src, tint) :: nil);
   fn_vars := nil;
-  fn_temps := ((_i, tint) :: (_j, tint) :: (_t'3, tint) :: (_t'2, tint) ::
-               (_t'1, tint) :: nil);
+  fn_temps := ((_i, tint) :: (_j, tint) :: (_t'2, tint) :: (_t'1, tint) ::
+               nil);
   fn_body :=
 (Ssequence
   (Ssequence
@@ -789,30 +348,30 @@ Definition f_print_graph := {|
                   Sskip
                   Sbreak)
                 (Ssequence
-                  (Sset _t'2
+                  (Sset _t'1
                     (Ederef
                       (Ebinop Oadd
                         (Ederef
                           (Ebinop Oadd
-                            (Evar _graph (tarray (tarray tint 8) 8))
+                            (Etempvar _graph (tptr (tarray tint 8)))
                             (Etempvar _i tint) (tptr (tarray tint 8)))
                           (tarray tint 8)) (Etempvar _j tint) (tptr tint))
                       tint))
-                  (Sifthenelse (Ebinop Oeq (Etempvar _t'2 tint)
+                  (Sifthenelse (Ebinop Oeq (Etempvar _t'1 tint)
                                  (Econst_int (Int.repr 2147483647) tint)
                                  tint)
                     (Scall None
                       (Evar _printf (Tfunction (Tcons (tptr tschar) Tnil)
                                       tint
                                       {|cc_vararg:=true; cc_unproto:=false; cc_structret:=false|}))
-                      ((Evar ___stringlit_5 (tarray tschar 3)) :: nil))
+                      ((Evar ___stringlit_2 (tarray tschar 3)) :: nil))
                     (Ssequence
-                      (Sset _t'3
+                      (Sset _t'2
                         (Ederef
                           (Ebinop Oadd
                             (Ederef
                               (Ebinop Oadd
-                                (Evar _graph (tarray (tarray tint 8) 8))
+                                (Etempvar _graph (tptr (tarray tint 8)))
                                 (Etempvar _i tint) (tptr (tarray tint 8)))
                               (tarray tint 8)) (Etempvar _j tint)
                             (tptr tint)) tint))
@@ -820,8 +379,8 @@ Definition f_print_graph := {|
                         (Evar _printf (Tfunction (Tcons (tptr tschar) Tnil)
                                         tint
                                         {|cc_vararg:=true; cc_unproto:=false; cc_structret:=false|}))
-                        ((Evar ___stringlit_2 (tarray tschar 4)) ::
-                         (Etempvar _t'3 tint) :: nil))))))
+                        ((Evar ___stringlit_1 (tarray tschar 4)) ::
+                         (Etempvar _t'2 tint) :: nil))))))
               (Sset _j
                 (Ebinop Oadd (Etempvar _j tint)
                   (Econst_int (Int.repr 1) tint) tint))))
@@ -831,320 +390,51 @@ Definition f_print_graph := {|
             ((Evar ___stringlit_3 (tarray tschar 2)) :: nil))))
       (Sset _i
         (Ebinop Oadd (Etempvar _i tint) (Econst_int (Int.repr 1) tint) tint))))
+  (Scall None
+    (Evar _printf (Tfunction (Tcons (tptr tschar) Tnil) tint
+                    {|cc_vararg:=true; cc_unproto:=false; cc_structret:=false|}))
+    ((Evar ___stringlit_4 (tarray tschar 13)) :: (Etempvar _src tint) :: nil)))
+|}.
+
+Definition f_printPath := {|
+  fn_return := tvoid;
+  fn_callconv := cc_default;
+  fn_params := ((_curr, tint) :: (_src, tint) :: (_prev, (tptr tint)) :: nil);
+  fn_vars := nil;
+  fn_temps := ((_t'1, tint) :: nil);
+  fn_body :=
+(Sifthenelse (Ebinop Oeq (Etempvar _curr tint) (Etempvar _src tint) tint)
+  (Scall None
+    (Evar _printf (Tfunction (Tcons (tptr tschar) Tnil) tint
+                    {|cc_vararg:=true; cc_unproto:=false; cc_structret:=false|}))
+    ((Evar ___stringlit_1 (tarray tschar 4)) :: (Etempvar _curr tint) :: nil))
   (Ssequence
-    (Sset _t'1 (Evar _src tint))
+    (Ssequence
+      (Sset _t'1
+        (Ederef
+          (Ebinop Oadd (Etempvar _prev (tptr tint)) (Etempvar _curr tint)
+            (tptr tint)) tint))
+      (Scall None
+        (Evar _printPath (Tfunction
+                           (Tcons tint (Tcons tint (Tcons (tptr tint) Tnil)))
+                           tvoid cc_default))
+        ((Etempvar _t'1 tint) :: (Etempvar _src tint) ::
+         (Etempvar _prev (tptr tint)) :: nil)))
     (Scall None
       (Evar _printf (Tfunction (Tcons (tptr tschar) Tnil) tint
                       {|cc_vararg:=true; cc_unproto:=false; cc_structret:=false|}))
-      ((Evar ___stringlit_6 (tarray tschar 13)) :: (Etempvar _t'1 tint) ::
+      ((Evar ___stringlit_1 (tarray tschar 4)) :: (Etempvar _curr tint) ::
        nil))))
-|}.
-
-Definition v_dist := {|
-  gvar_info := (tarray tint 8);
-  gvar_init := (Init_space 32 :: nil);
-  gvar_readonly := false;
-  gvar_volatile := false
-|}.
-
-Definition v_prev := {|
-  gvar_info := (tarray tint 8);
-  gvar_init := (Init_space 32 :: nil);
-  gvar_readonly := false;
-  gvar_volatile := false
-|}.
-
-Definition f_dijkstra := {|
-  fn_return := tvoid;
-  fn_callconv := cc_default;
-  fn_params := nil;
-  fn_vars := ((_pq, (tptr (Tstruct _Node noattr))) :: nil);
-  fn_temps := ((_i, tint) :: (_u, tint) :: (_t'2, tint) :: (_t'1, tint) ::
-               (_t'13, tint) :: (_t'12, tint) ::
-               (_t'11, (tptr (Tstruct _Node noattr))) :: (_t'10, tint) ::
-               (_t'9, tint) :: (_t'8, tint) :: (_t'7, tint) ::
-               (_t'6, tint) :: (_t'5, tint) :: (_t'4, tint) ::
-               (_t'3, tint) :: nil);
-  fn_body :=
-(Ssequence
-  (Sassign (Evar _pq (tptr (Tstruct _Node noattr)))
-    (Ecast (Econst_int (Int.repr 0) tint) (tptr tvoid)))
-  (Ssequence
-    (Ssequence
-      (Sset _i (Econst_int (Int.repr 0) tint))
-      (Sloop
-        (Ssequence
-          (Sifthenelse (Ebinop Olt (Etempvar _i tint)
-                         (Econst_int (Int.repr 8) tint) tint)
-            Sskip
-            Sbreak)
-          (Ssequence
-            (Ssequence
-              (Ssequence
-                (Sset _t'13 (Evar _src tint))
-                (Sifthenelse (Ebinop Oeq (Etempvar _i tint)
-                               (Etempvar _t'13 tint) tint)
-                  (Sset _t'1 (Ecast (Econst_int (Int.repr 0) tint) tint))
-                  (Sset _t'1
-                    (Ecast (Econst_int (Int.repr 2147483647) tint) tint))))
-              (Sassign
-                (Ederef
-                  (Ebinop Oadd (Evar _dist (tarray tint 8))
-                    (Etempvar _i tint) (tptr tint)) tint)
-                (Etempvar _t'1 tint)))
-            (Ssequence
-              (Sassign
-                (Ederef
-                  (Ebinop Oadd (Evar _prev (tarray tint 8))
-                    (Etempvar _i tint) (tptr tint)) tint)
-                (Econst_int (Int.repr 2147483647) tint))
-              (Ssequence
-                (Sset _t'12
-                  (Ederef
-                    (Ebinop Oadd (Evar _dist (tarray tint 8))
-                      (Etempvar _i tint) (tptr tint)) tint))
-                (Scall None
-                  (Evar _push (Tfunction
-                                (Tcons tint
-                                  (Tcons tint
-                                    (Tcons
-                                      (tptr (tptr (Tstruct _Node noattr)))
-                                      Tnil))) tvoid cc_default))
-                  ((Etempvar _i tint) :: (Etempvar _t'12 tint) ::
-                   (Eaddrof (Evar _pq (tptr (Tstruct _Node noattr)))
-                     (tptr (tptr (Tstruct _Node noattr)))) :: nil))))))
-        (Sset _i
-          (Ebinop Oadd (Etempvar _i tint) (Econst_int (Int.repr 1) tint)
-            tint))))
-    (Sloop
-      (Ssequence
-        (Ssequence
-          (Sset _t'11 (Evar _pq (tptr (Tstruct _Node noattr))))
-          (Sifthenelse (Ebinop One
-                         (Etempvar _t'11 (tptr (Tstruct _Node noattr)))
-                         (Ecast (Econst_int (Int.repr 0) tint) (tptr tvoid))
-                         tint)
-            Sskip
-            Sbreak))
-        (Ssequence
-          (Ssequence
-            (Scall (Some _t'2)
-              (Evar _popMin (Tfunction
-                              (Tcons (tptr (tptr (Tstruct _Node noattr)))
-                                Tnil) tint cc_default))
-              ((Eaddrof (Evar _pq (tptr (Tstruct _Node noattr)))
-                 (tptr (tptr (Tstruct _Node noattr)))) :: nil))
-            (Sset _u (Etempvar _t'2 tint)))
-          (Ssequence
-            (Sifthenelse (Ebinop Olt (Etempvar _u tint)
-                           (Econst_int (Int.repr 0) tint) tint)
-              Sbreak
-              Sskip)
-            (Ssequence
-              (Sset _i (Econst_int (Int.repr 0) tint))
-              (Sloop
-                (Ssequence
-                  (Sifthenelse (Ebinop Olt (Etempvar _i tint)
-                                 (Econst_int (Int.repr 8) tint) tint)
-                    Sskip
-                    Sbreak)
-                  (Ssequence
-                    (Sset _t'3
-                      (Ederef
-                        (Ebinop Oadd
-                          (Ederef
-                            (Ebinop Oadd
-                              (Evar _graph (tarray (tarray tint 8) 8))
-                              (Etempvar _u tint) (tptr (tarray tint 8)))
-                            (tarray tint 8)) (Etempvar _i tint) (tptr tint))
-                        tint))
-                    (Sifthenelse (Ebinop Olt (Etempvar _t'3 tint)
-                                   (Econst_int (Int.repr 2147483647) tint)
-                                   tint)
-                      (Ssequence
-                        (Sset _t'4
-                          (Ederef
-                            (Ebinop Oadd (Evar _dist (tarray tint 8))
-                              (Etempvar _i tint) (tptr tint)) tint))
-                        (Ssequence
-                          (Sset _t'5
-                            (Ederef
-                              (Ebinop Oadd (Evar _dist (tarray tint 8))
-                                (Etempvar _u tint) (tptr tint)) tint))
-                          (Ssequence
-                            (Sset _t'6
-                              (Ederef
-                                (Ebinop Oadd
-                                  (Ederef
-                                    (Ebinop Oadd
-                                      (Evar _graph (tarray (tarray tint 8) 8))
-                                      (Etempvar _u tint)
-                                      (tptr (tarray tint 8)))
-                                    (tarray tint 8)) (Etempvar _i tint)
-                                  (tptr tint)) tint))
-                            (Sifthenelse (Ebinop Ogt (Etempvar _t'4 tint)
-                                           (Ebinop Oadd (Etempvar _t'5 tint)
-                                             (Etempvar _t'6 tint) tint) tint)
-                              (Ssequence
-                                (Ssequence
-                                  (Sset _t'9
-                                    (Ederef
-                                      (Ebinop Oadd
-                                        (Evar _dist (tarray tint 8))
-                                        (Etempvar _u tint) (tptr tint)) tint))
-                                  (Ssequence
-                                    (Sset _t'10
-                                      (Ederef
-                                        (Ebinop Oadd
-                                          (Ederef
-                                            (Ebinop Oadd
-                                              (Evar _graph (tarray (tarray tint 8) 8))
-                                              (Etempvar _u tint)
-                                              (tptr (tarray tint 8)))
-                                            (tarray tint 8))
-                                          (Etempvar _i tint) (tptr tint))
-                                        tint))
-                                    (Sassign
-                                      (Ederef
-                                        (Ebinop Oadd
-                                          (Evar _dist (tarray tint 8))
-                                          (Etempvar _i tint) (tptr tint))
-                                        tint)
-                                      (Ebinop Oadd (Etempvar _t'9 tint)
-                                        (Etempvar _t'10 tint) tint))))
-                                (Ssequence
-                                  (Sassign
-                                    (Ederef
-                                      (Ebinop Oadd
-                                        (Evar _prev (tarray tint 8))
-                                        (Etempvar _i tint) (tptr tint)) tint)
-                                    (Etempvar _u tint))
-                                  (Ssequence
-                                    (Ssequence
-                                      (Sset _t'8
-                                        (Ederef
-                                          (Ebinop Oadd
-                                            (Evar _dist (tarray tint 8))
-                                            (Etempvar _i tint) (tptr tint))
-                                          tint))
-                                      (Scall None
-                                        (Evar _adjustWeight (Tfunction
-                                                              (Tcons tint
-                                                                (Tcons tint
-                                                                  (Tcons
-                                                                    (tptr (tptr (Tstruct _Node noattr)))
-                                                                    Tnil)))
-                                                              tvoid
-                                                              cc_default))
-                                        ((Etempvar _i tint) ::
-                                         (Etempvar _t'8 tint) ::
-                                         (Eaddrof
-                                           (Evar _pq (tptr (Tstruct _Node noattr)))
-                                           (tptr (tptr (Tstruct _Node noattr)))) ::
-                                         nil)))
-                                    (Ssequence
-                                      (Sset _t'7
-                                        (Ederef
-                                          (Ebinop Oadd
-                                            (Evar _dist (tarray tint 8))
-                                            (Etempvar _i tint) (tptr tint))
-                                          tint))
-                                      (Scall None
-                                        (Evar _printf (Tfunction
-                                                        (Tcons (tptr tschar)
-                                                          Tnil) tint
-                                                        {|cc_vararg:=true; cc_unproto:=false; cc_structret:=false|}))
-                                        ((Evar ___stringlit_7 (tarray tschar 45)) ::
-                                         (Etempvar _i tint) ::
-                                         (Etempvar _t'7 tint) :: nil))))))
-                              Sskip))))
-                      Sskip)))
-                (Sset _i
-                  (Ebinop Oadd (Etempvar _i tint)
-                    (Econst_int (Int.repr 1) tint) tint)))))))
-      Sskip)))
-|}.
-
-Definition f_getPath := {|
-  fn_return := tvoid;
-  fn_callconv := cc_default;
-  fn_params := ((_dst__1, tint) :: nil);
-  fn_vars := ((_pq, (tptr (Tstruct _Node noattr))) :: nil);
-  fn_temps := ((_before, tint) :: (_t'1, tint) :: (_t'6, tint) ::
-               (_t'5, tint) :: (_t'4, tint) :: (_t'3, tint) ::
-               (_t'2, (tptr (Tstruct _Node noattr))) :: nil);
-  fn_body :=
-(Ssequence
-  (Ssequence
-    (Sset _t'5 (Evar _src tint))
-    (Sifthenelse (Ebinop One (Etempvar _dst__1 tint) (Etempvar _t'5 tint)
-                   tint)
-      (Ssequence
-        (Sset _t'6
-          (Ederef
-            (Ebinop Oadd (Evar _dist (tarray tint 8)) (Etempvar _dst__1 tint)
-              (tptr tint)) tint))
-        (Sset _t'1
-          (Ecast
-            (Ebinop Olt (Etempvar _t'6 tint)
-              (Econst_int (Int.repr 2147483647) tint) tint) tbool)))
-      (Sset _t'1 (Econst_int (Int.repr 0) tint))))
-  (Sifthenelse (Etempvar _t'1 tint)
-    (Ssequence
-      (Ssequence
-        (Sset _t'3 (Evar _src tint))
-        (Ssequence
-          (Sset _t'4
-            (Ederef
-              (Ebinop Oadd (Evar _dist (tarray tint 8))
-                (Etempvar _dst__1 tint) (tptr tint)) tint))
-          (Scall None
-            (Evar _printf (Tfunction (Tcons (tptr tschar) Tnil) tint
-                            {|cc_vararg:=true; cc_unproto:=false; cc_structret:=false|}))
-            ((Evar ___stringlit_8 (tarray tschar 38)) ::
-             (Etempvar _t'3 tint) :: (Etempvar _dst__1 tint) ::
-             (Etempvar _t'4 tint) :: nil))))
-      (Ssequence
-        (Sassign (Evar _pq (tptr (Tstruct _Node noattr)))
-          (Ecast (Econst_int (Int.repr 0) tint) (tptr tvoid)))
-        (Ssequence
-          (Sset _before (Etempvar _dst__1 tint))
-          (Ssequence
-            (Swhile
-              (Ebinop Olt (Etempvar _before tint)
-                (Econst_int (Int.repr 2147483647) tint) tint)
-              (Ssequence
-                (Scall None
-                  (Evar _push (Tfunction
-                                (Tcons tint
-                                  (Tcons tint
-                                    (Tcons
-                                      (tptr (tptr (Tstruct _Node noattr)))
-                                      Tnil))) tvoid cc_default))
-                  ((Etempvar _before tint) ::
-                   (Econst_int (Int.repr 0) tint) ::
-                   (Eaddrof (Evar _pq (tptr (Tstruct _Node noattr)))
-                     (tptr (tptr (Tstruct _Node noattr)))) :: nil))
-                (Sset _before
-                  (Ederef
-                    (Ebinop Oadd (Evar _prev (tarray tint 8))
-                      (Etempvar _before tint) (tptr tint)) tint))))
-            (Ssequence
-              (Sset _t'2 (Evar _pq (tptr (Tstruct _Node noattr))))
-              (Scall None
-                (Evar _print_verts (Tfunction
-                                     (Tcons (tptr (Tstruct _Node noattr))
-                                       Tnil) tvoid cc_default))
-                ((Etempvar _t'2 (tptr (Tstruct _Node noattr))) :: nil)))))))
-    Sskip))
 |}.
 
 Definition f_getPaths := {|
   fn_return := tvoid;
   fn_callconv := cc_default;
-  fn_params := nil;
+  fn_params := ((_src, tint) :: (_dist, (tptr tint)) ::
+                (_prev, (tptr tint)) :: nil);
   fn_vars := nil;
-  fn_temps := ((_i, tint) :: (_t'1, tint) :: nil);
+  fn_temps := ((_i, tint) :: (_t'1, tint) :: (_t'3, tint) :: (_t'2, tint) ::
+               nil);
   fn_body :=
 (Ssequence
   (Sset _i (Econst_int (Int.repr 0) tint))
@@ -1155,61 +445,283 @@ Definition f_getPaths := {|
         Sskip
         Sbreak)
       (Ssequence
-        (Sset _t'1
-          (Ederef
-            (Ebinop Oadd (Evar _dist (tarray tint 8)) (Etempvar _i tint)
-              (tptr tint)) tint))
-        (Sifthenelse (Ebinop Olt (Etempvar _t'1 tint)
-                       (Econst_int (Int.repr 2147483647) tint) tint)
-          (Scall None
-            (Evar _getPath (Tfunction (Tcons tint Tnil) tvoid cc_default))
-            ((Etempvar _i tint) :: nil))
-          (Scall None
-            (Evar _printf (Tfunction (Tcons (tptr tschar) Tnil) tint
-                            {|cc_vararg:=true; cc_unproto:=false; cc_structret:=false|}))
-            ((Evar ___stringlit_9 (tarray tschar 38)) ::
-             (Etempvar _i tint) :: nil)))))
+        (Sifthenelse (Ebinop One (Etempvar _i tint) (Etempvar _src tint)
+                       tint)
+          (Ssequence
+            (Sset _t'3
+              (Ederef
+                (Ebinop Oadd (Etempvar _dist (tptr tint)) (Etempvar _i tint)
+                  (tptr tint)) tint))
+            (Sset _t'1
+              (Ecast
+                (Ebinop Olt (Etempvar _t'3 tint)
+                  (Econst_int (Int.repr 2147483647) tint) tint) tbool)))
+          (Sset _t'1 (Econst_int (Int.repr 0) tint)))
+        (Sifthenelse (Etempvar _t'1 tint)
+          (Ssequence
+            (Ssequence
+              (Sset _t'2
+                (Ederef
+                  (Ebinop Oadd (Etempvar _dist (tptr tint))
+                    (Etempvar _i tint) (tptr tint)) tint))
+              (Scall None
+                (Evar _printf (Tfunction (Tcons (tptr tschar) Tnil) tint
+                                {|cc_vararg:=true; cc_unproto:=false; cc_structret:=false|}))
+                ((Evar ___stringlit_5 (tarray tschar 39)) ::
+                 (Etempvar _src tint) :: (Etempvar _i tint) ::
+                 (Etempvar _t'2 tint) :: nil)))
+            (Scall None
+              (Evar _printPath (Tfunction
+                                 (Tcons tint
+                                   (Tcons tint (Tcons (tptr tint) Tnil)))
+                                 tvoid cc_default))
+              ((Etempvar _i tint) :: (Etempvar _src tint) ::
+               (Etempvar _prev (tptr tint)) :: nil)))
+          Sskip)))
     (Sset _i
       (Ebinop Oadd (Etempvar _i tint) (Econst_int (Int.repr 1) tint) tint))))
+|}.
+
+Definition f_dijkstra := {|
+  fn_return := tvoid;
+  fn_callconv := cc_default;
+  fn_params := ((_graph, (tptr (tarray tint 8))) :: (_src, tint) ::
+                (_dist, (tptr tint)) :: (_prev, (tptr tint)) :: nil);
+  fn_vars := ((_pq, (tarray tint 8)) :: nil);
+  fn_temps := ((_i, tint) :: (_j, tint) :: (_u, tint) :: (_t'1, tint) ::
+               (_t'9, tint) :: (_t'8, tint) :: (_t'7, tint) ::
+               (_t'6, tint) :: (_t'5, tint) :: (_t'4, tint) ::
+               (_t'3, tint) :: (_t'2, tint) :: nil);
+  fn_body :=
+(Ssequence
+  (Ssequence
+    (Sset _i (Econst_int (Int.repr 0) tint))
+    (Sloop
+      (Ssequence
+        (Sifthenelse (Ebinop Olt (Etempvar _i tint)
+                       (Econst_int (Int.repr 8) tint) tint)
+          Sskip
+          Sbreak)
+        (Ssequence
+          (Sassign
+            (Ederef
+              (Ebinop Oadd (Etempvar _dist (tptr tint)) (Etempvar _i tint)
+                (tptr tint)) tint) (Econst_int (Int.repr 2147483647) tint))
+          (Ssequence
+            (Sassign
+              (Ederef
+                (Ebinop Oadd (Etempvar _prev (tptr tint)) (Etempvar _i tint)
+                  (tptr tint)) tint) (Econst_int (Int.repr 2147483647) tint))
+            (Ssequence
+              (Sset _t'9
+                (Ederef
+                  (Ebinop Oadd (Etempvar _dist (tptr tint))
+                    (Etempvar _i tint) (tptr tint)) tint))
+              (Sassign
+                (Ederef
+                  (Ebinop Oadd (Evar _pq (tarray tint 8)) (Etempvar _i tint)
+                    (tptr tint)) tint) (Etempvar _t'9 tint))))))
+      (Sset _i
+        (Ebinop Oadd (Etempvar _i tint) (Econst_int (Int.repr 1) tint) tint))))
+  (Ssequence
+    (Sassign
+      (Ederef
+        (Ebinop Oadd (Etempvar _dist (tptr tint)) (Etempvar _src tint)
+          (tptr tint)) tint) (Econst_int (Int.repr 0) tint))
+    (Ssequence
+      (Sassign
+        (Ederef
+          (Ebinop Oadd (Evar _pq (tarray tint 8)) (Etempvar _src tint)
+            (tptr tint)) tint) (Econst_int (Int.repr 0) tint))
+      (Ssequence
+        (Sassign
+          (Ederef
+            (Ebinop Oadd (Etempvar _prev (tptr tint)) (Etempvar _src tint)
+              (tptr tint)) tint) (Etempvar _src tint))
+        (Ssequence
+          (Sset _j (Econst_int (Int.repr 0) tint))
+          (Sloop
+            (Ssequence
+              (Sifthenelse (Ebinop Olt (Etempvar _j tint)
+                             (Econst_int (Int.repr 8) tint) tint)
+                Sskip
+                Sbreak)
+              (Ssequence
+                (Ssequence
+                  (Scall (Some _t'1)
+                    (Evar _popMin (Tfunction (Tcons (tptr tint) Tnil) tint
+                                    cc_default))
+                    ((Evar _pq (tarray tint 8)) :: nil))
+                  (Sset _u (Etempvar _t'1 tint)))
+                (Ssequence
+                  (Sifthenelse (Ebinop Oeq (Etempvar _u tint)
+                                 (Eunop Oneg (Econst_int (Int.repr 1) tint)
+                                   tint) tint)
+                    Sbreak
+                    Sskip)
+                  (Ssequence
+                    (Sset _i (Econst_int (Int.repr 0) tint))
+                    (Sloop
+                      (Ssequence
+                        (Sifthenelse (Ebinop Olt (Etempvar _i tint)
+                                       (Econst_int (Int.repr 8) tint) tint)
+                          Sskip
+                          Sbreak)
+                        (Ssequence
+                          (Sset _t'2
+                            (Ederef
+                              (Ebinop Oadd
+                                (Ederef
+                                  (Ebinop Oadd
+                                    (Etempvar _graph (tptr (tarray tint 8)))
+                                    (Etempvar _u tint)
+                                    (tptr (tarray tint 8))) (tarray tint 8))
+                                (Etempvar _i tint) (tptr tint)) tint))
+                          (Sifthenelse (Ebinop Olt (Etempvar _t'2 tint)
+                                         (Econst_int (Int.repr 2147483647) tint)
+                                         tint)
+                            (Ssequence
+                              (Sset _t'3
+                                (Ederef
+                                  (Ebinop Oadd (Etempvar _dist (tptr tint))
+                                    (Etempvar _i tint) (tptr tint)) tint))
+                              (Ssequence
+                                (Sset _t'4
+                                  (Ederef
+                                    (Ebinop Oadd (Etempvar _dist (tptr tint))
+                                      (Etempvar _u tint) (tptr tint)) tint))
+                                (Ssequence
+                                  (Sset _t'5
+                                    (Ederef
+                                      (Ebinop Oadd
+                                        (Ederef
+                                          (Ebinop Oadd
+                                            (Etempvar _graph (tptr (tarray tint 8)))
+                                            (Etempvar _u tint)
+                                            (tptr (tarray tint 8)))
+                                          (tarray tint 8)) (Etempvar _i tint)
+                                        (tptr tint)) tint))
+                                  (Sifthenelse (Ebinop Ogt
+                                                 (Etempvar _t'3 tint)
+                                                 (Ebinop Oadd
+                                                   (Etempvar _t'4 tint)
+                                                   (Etempvar _t'5 tint) tint)
+                                                 tint)
+                                    (Ssequence
+                                      (Ssequence
+                                        (Sset _t'7
+                                          (Ederef
+                                            (Ebinop Oadd
+                                              (Etempvar _dist (tptr tint))
+                                              (Etempvar _u tint) (tptr tint))
+                                            tint))
+                                        (Ssequence
+                                          (Sset _t'8
+                                            (Ederef
+                                              (Ebinop Oadd
+                                                (Ederef
+                                                  (Ebinop Oadd
+                                                    (Etempvar _graph (tptr (tarray tint 8)))
+                                                    (Etempvar _u tint)
+                                                    (tptr (tarray tint 8)))
+                                                  (tarray tint 8))
+                                                (Etempvar _i tint)
+                                                (tptr tint)) tint))
+                                          (Sassign
+                                            (Ederef
+                                              (Ebinop Oadd
+                                                (Etempvar _dist (tptr tint))
+                                                (Etempvar _i tint)
+                                                (tptr tint)) tint)
+                                            (Ebinop Oadd (Etempvar _t'7 tint)
+                                              (Etempvar _t'8 tint) tint))))
+                                      (Ssequence
+                                        (Sassign
+                                          (Ederef
+                                            (Ebinop Oadd
+                                              (Etempvar _prev (tptr tint))
+                                              (Etempvar _i tint) (tptr tint))
+                                            tint) (Etempvar _u tint))
+                                        (Ssequence
+                                          (Sset _t'6
+                                            (Ederef
+                                              (Ebinop Oadd
+                                                (Etempvar _dist (tptr tint))
+                                                (Etempvar _i tint)
+                                                (tptr tint)) tint))
+                                          (Sassign
+                                            (Ederef
+                                              (Ebinop Oadd
+                                                (Evar _pq (tarray tint 8))
+                                                (Etempvar _i tint)
+                                                (tptr tint)) tint)
+                                            (Etempvar _t'6 tint)))))
+                                    Sskip))))
+                            Sskip)))
+                      (Sset _i
+                        (Ebinop Oadd (Etempvar _i tint)
+                          (Econst_int (Int.repr 1) tint) tint)))))))
+            (Sset _j
+              (Ebinop Oadd (Etempvar _j tint) (Econst_int (Int.repr 1) tint)
+                tint))))))))
 |}.
 
 Definition f_main := {|
   fn_return := tint;
   fn_callconv := cc_default;
   fn_params := ((_argc, tint) :: (_argv, (tptr (tptr tschar))) :: nil);
-  fn_vars := nil;
-  fn_temps := nil;
+  fn_vars := ((_graph, (tarray (tarray tint 8) 8)) ::
+              (_prev, (tarray tint 8)) :: (_dist, (tarray tint 8)) :: nil);
+  fn_temps := ((_i, tint) :: (_j, tint) :: (_src, tint) :: nil);
   fn_body :=
 (Ssequence
   (Ssequence
-    (Scall None (Evar _setup (Tfunction Tnil tvoid cc_default)) nil)
+    (Sset _src (Econst_int (Int.repr 0) tint))
     (Ssequence
-      (Scall None (Evar _print_graph (Tfunction Tnil tvoid cc_default)) nil)
+      (Scall None
+        (Evar _setup (Tfunction (Tcons (tptr (tarray tint 8)) Tnil) tvoid
+                       cc_default))
+        ((Evar _graph (tarray (tarray tint 8) 8)) :: nil))
       (Ssequence
-        (Scall None (Evar _dijkstra (Tfunction Tnil tvoid cc_default)) nil)
+        (Scall None
+          (Evar _print_graph (Tfunction
+                               (Tcons (tptr (tarray tint 8))
+                                 (Tcons tint Tnil)) tvoid cc_default))
+          ((Evar _graph (tarray (tarray tint 8) 8)) ::
+           (Etempvar _src tint) :: nil))
         (Ssequence
-          (Scall None (Evar _getPaths (Tfunction Tnil tvoid cc_default)) nil)
-          (Sreturn (Some (Econst_int (Int.repr 0) tint)))))))
+          (Scall None
+            (Evar _dijkstra (Tfunction
+                              (Tcons (tptr (tarray tint 8))
+                                (Tcons tint
+                                  (Tcons (tptr tint)
+                                    (Tcons (tptr tint) Tnil)))) tvoid
+                              cc_default))
+            ((Evar _graph (tarray (tarray tint 8) 8)) ::
+             (Etempvar _src tint) :: (Evar _dist (tarray tint 8)) ::
+             (Evar _prev (tarray tint 8)) :: nil))
+          (Ssequence
+            (Scall None
+              (Evar _getPaths (Tfunction
+                                (Tcons tint
+                                  (Tcons (tptr tint)
+                                    (Tcons (tptr tint) Tnil))) tvoid
+                                cc_default))
+              ((Etempvar _src tint) :: (Evar _dist (tarray tint 8)) ::
+               (Evar _prev (tarray tint 8)) :: nil))
+            (Sreturn (Some (Econst_int (Int.repr 0) tint))))))))
   (Sreturn (Some (Econst_int (Int.repr 0) tint))))
 |}.
 
 Definition composites : list composite_definition :=
-(Composite _Node Struct
-   ((_vertex, tint) :: (_weight, tint) ::
-    (_next, (tptr (Tstruct _Node noattr))) ::
-    (_prev, (tptr (Tstruct _Node noattr))) :: nil)
-   noattr :: nil).
+nil.
 
 Definition global_definitions : list (ident * globdef fundef type) :=
-((___stringlit_1, Gvar v___stringlit_1) ::
- (___stringlit_6, Gvar v___stringlit_6) ::
- (___stringlit_7, Gvar v___stringlit_7) ::
- (___stringlit_9, Gvar v___stringlit_9) ::
- (___stringlit_2, Gvar v___stringlit_2) ::
- (___stringlit_3, Gvar v___stringlit_3) ::
- (___stringlit_4, Gvar v___stringlit_4) ::
+((___stringlit_4, Gvar v___stringlit_4) ::
  (___stringlit_5, Gvar v___stringlit_5) ::
- (___stringlit_8, Gvar v___stringlit_8) ::
+ (___stringlit_1, Gvar v___stringlit_1) ::
+ (___stringlit_3, Gvar v___stringlit_3) ::
+ (___stringlit_2, Gvar v___stringlit_2) ::
  (___builtin_bswap,
    Gfun(External (EF_builtin "__builtin_bswap"
                    (mksignature (AST.Tint :: nil) (Some AST.Tint) cc_default))
@@ -1451,9 +963,6 @@ Definition global_definitions : list (ident * globdef fundef type) :=
                      {|cc_vararg:=true; cc_unproto:=false; cc_structret:=false|}))
      (Tcons tint Tnil) tvoid
      {|cc_vararg:=true; cc_unproto:=false; cc_structret:=false|})) ::
- (_malloc,
-   Gfun(External EF_malloc (Tcons tuint Tnil) (tptr tvoid) cc_default)) ::
- (_free, Gfun(External EF_free (Tcons (tptr tvoid) Tnil) tvoid cc_default)) ::
  (_rand,
    Gfun(External (EF_external "rand"
                    (mksignature nil (Some AST.Tint) cc_default)) Tnil tint
@@ -1472,26 +981,19 @@ Definition global_definitions : list (ident * globdef fundef type) :=
    Gfun(External (EF_external "time"
                    (mksignature (AST.Tint :: nil) (Some AST.Tint) cc_default))
      (Tcons (tptr tint) Tnil) tint cc_default)) ::
- (_push, Gfun(Internal f_push)) ::
- (_deleteNode, Gfun(Internal f_deleteNode)) ::
  (_popMin, Gfun(Internal f_popMin)) ::
- (_adjustWeight, Gfun(Internal f_adjustWeight)) ::
- (_print_verts, Gfun(Internal f_print_verts)) ::
- (_print_list, Gfun(Internal f_print_list)) :: (_graph, Gvar v_graph) ::
- (_src, Gvar v_src) :: (_dst, Gvar v_dst) ::
+ (_pq_not_emp, Gfun(Internal f_pq_not_emp)) ::
  (_setup, Gfun(Internal f_setup)) ::
- (_print_graph, Gfun(Internal f_print_graph)) :: (_dist, Gvar v_dist) ::
- (_prev, Gvar v_prev) :: (_dijkstra, Gfun(Internal f_dijkstra)) ::
- (_getPath, Gfun(Internal f_getPath)) ::
- (_getPaths, Gfun(Internal f_getPaths)) :: (_main, Gfun(Internal f_main)) ::
+ (_print_graph, Gfun(Internal f_print_graph)) ::
+ (_printPath, Gfun(Internal f_printPath)) ::
+ (_getPaths, Gfun(Internal f_getPaths)) ::
+ (_dijkstra, Gfun(Internal f_dijkstra)) :: (_main, Gfun(Internal f_main)) ::
  nil).
 
 Definition public_idents : list ident :=
-(_main :: _getPaths :: _getPath :: _dijkstra :: _prev :: _dist ::
- _print_graph :: _setup :: _dst :: _src :: _graph :: _print_list ::
- _print_verts :: _adjustWeight :: _popMin :: _deleteNode :: _push :: _time ::
- _printf :: _srand :: _rand :: _free :: _malloc :: ___builtin_debug ::
- ___builtin_nop :: ___builtin_write32_reversed ::
+(_main :: _dijkstra :: _getPaths :: _printPath :: _print_graph :: _setup ::
+ _pq_not_emp :: _popMin :: _time :: _printf :: _srand :: _rand ::
+ ___builtin_debug :: ___builtin_nop :: ___builtin_write32_reversed ::
  ___builtin_write16_reversed :: ___builtin_read32_reversed ::
  ___builtin_read16_reversed :: ___builtin_fnmsub :: ___builtin_fnmadd ::
  ___builtin_fmsub :: ___builtin_fmadd :: ___builtin_fmin ::
