sample_mark/verif_dijkstra.v
@@ -11,48 +11,131 @@ Require Import RamifyCoq.msl_application.DijkstraArrayGraph.
 Require Import RamifyCoq.sample_mark.spatial_dijkstra_array_graph.
 Require Import Coq.omega.Omega.
 Require Import Coq.Lists.List.
+Definition inf := 2147483647.
+
 
 Definition whole_graph sh g x := (@graph_rep_spatial mpred pointer_val (SDAG_VST sh) g x).
 
-(* Spec:  *)
-(* 	\exists mypath. path_ends g mypath src dst, *)
-(* 		\forall path. path_ends g path src dest ->  *)
-(* 			path_cost path <= past_cost mypath -> *)
-(* 				mypath = path *)
+Fixpoint create_path (src dst : VType) (prev : list VType) (ans : list VType) (n : nat) : list VType :=
+  match n with
+  | O => ans
+  | S n' => if Z.eq_dec src dst
+            then src :: ans
+            else create_path src (Znth dst prev) prev (dst :: ans) n'
+  end.
 
+(*
+sample prev array, where src = 3, dst = 8.
+[inf;  3 ; inf;  3 ;  5 ;  1 ;  1 ; inf;  6 ]
+  0    1    2    3    4    5    6    7    8     <- indices
 
-Definition dijkstra_correct (g: Graph) p src dst : Prop :=
+prev[3] = 3, which indicates that 3 is the source.
+
+The above function create_path will work only if 
+the prev array has been generated perfectly. ie, 
+(1) There needs to be some cell such that its value is the same as its index. 
+(2) There need to be no loops. 
+(3) If I query any cell, its value needs to be either 
+   (a) inf (meaning the cell was unreachable)
+  or
+   (b) it needs to point to another cell such that that cell will lead me closer to the source.
+
+If all these guarantees are set up, then I can find you the 
+source.  *)
+
+Definition dijkstra_correct (g: Graph) (src : VType) (prev: list VType) : Prop :=
+  forall dst,
+    (Znth dst prev) = inf \/ (* unreachable *)
+    let p := (src, create_path src dst prev [] 8) in
+    valid_path g p ->
     path_ends g p src dst ->
-    forall p', path_ends g p' src dst ->
+    forall p', valid_path g p' ->
+               path_ends g p' src dst ->
                Nat.lt (path_cost g p') (path_cost g p) ->
                p = p'.
-         
+
 Definition dijkstra_spec :=
   DECLARE _dijkstra
-  WITH sh: wshare, g: Graph, arr: pointer_val,
-       dist: pointer_val, prev: pointer_val,
-       i: Z, src: Z, dst: Z
-  PRE []
-    PROP ()
-    LOCAL () (* temp _pq (pointer_val_val arr); temp _i (Vint (Int.repr i))) *)
-    SEP (whole_graph sh g arr)
+  WITH sh: wshare, g: Graph, arr : pointer_val,
+       dist : pointer_val, prev : pointer_val, src : Z
+  PRE [_graph OF (tptr (tarray tint 8)), _src OF tint,
+       _dist OF (tptr tint), _prev OF (tptr tint)]
+  PROP (0 <= src < 8)
+  LOCAL (temp _graph (pointer_val_val arr);
+         temp _src (Vint (Int.repr src));
+         temp _dist (pointer_val_val dist);
+         temp _prev (pointer_val_val prev))
+  SEP (whole_graph sh g arr;
+       data_at_ Tsh (tarray tint 8) (pointer_val_val dist);
+       data_at_ Tsh (tarray tint 8) (pointer_val_val prev))
   POST [tvoid]
-      EX p : (@path VType EType),
-      PROP (dijkstra_correct g p src dst)
+      EX prev : list Z, (* should probably go away *)
+      PROP (dijkstra_correct g src prev)
       LOCAL ()
       SEP (whole_graph sh g arr).
 
 Definition Gprog : funspecs := ltac:(with_library prog [dijkstra_spec]).
 
-Lemma body_find: semax_body Vprog Gprog f_dijkstra dijkstra_spec.
+Lemma body_dijkstra: semax_body Vprog Gprog f_dijkstra dijkstra_spec.
 Proof.
-  start_function.
-  forward.
-  forward_for_simple_bound 8 
-    (EX i: Z,
-    PROP  ()
-    LOCAL (lvar _pq (tptr (Tstruct _Node noattr)) v_pq)
-    SEP (data_at Tsh (tptr (Tstruct _Node noattr)) (Vint (Int.repr 0)) v_pq;
-         whole_graph sh g arr)).
+  start_function. 
+  forward_for_simple_bound
+    8
+    (EX i : Z,
+     PROP ()
+     LOCAL (lvar _pq (tarray tint 8) v_pq; lvar _prev (tarray tint 8) v_prev;
+            lvar _dist (tarray tint 8) v_dist;
+            temp _src (Vint (Int.repr src));
+           temp _j (Vint (Int.repr j)))
+     SEP (data_at_ Tsh (tarray tint 8) v_pq *
+          data_at_ Tsh (tarray tint 8) (pointer_val_val prev) *
+          data_at_ Tsh (tarray tint 8) (v_prev) *
+          data_at_ Tsh (tarray tint 8) (pointer_val_val dist) *
+          data_at_ Tsh (tarray tint 8) (v_dist) *
+          whole_graph sh g arr)).
   - entailer!.
-    Abort.
+  - Intros. do 3 forward. 2: forward; entailer!. 
+    entailer!.
+    rewrite upd_Znth_Zlength in H5.
+    rewrite <- H5 in H1.
+    rewrite upd_Znth_same. 2, 3: assumption.
+    apply is_int_I32_Vint.
+  - Intros. forward. forward.
+    forward_loop
+      (
+        EX j : Z,
+        PROP ()
+        LOCAL (lvar _pq (tarray tint 8) v_pq; temp _j (Vint (Int.repr j)))
+        SEP (data_at Tsh (tarray tint 8)
+            (upd_Znth src (default_val (tarray tint 8)) (Vint (Int.repr 0))) v_pq;
+     data_at_ Tsh (tarray tint 8) v_prev;
+     data_at Tsh (tarray tint 8)
+       (upd_Znth src (default_val (tarray tint 8)) (Vint (Int.repr 0))) v_dist;
+     whole_graph sh g arr)
+      )
+      break:
+      (
+        PROP ()
+        LOCAL ()
+        SEP ()
+      ).
+    + forward. entailer!.
+
+
+
+
+
+
+
+
+
+
+      
+      admit.
+      admit.
+    + forward_if.
+      * admit.
+      * forward. admit.
+    + unfold POSTCONDITION. unfold abbreviate.
+      admit.
+Admitted.
